CLEAN features and improvements
- improved boilerplate
- instantiation of thread_info (#164)
- new implementation of use_module
- removing tlocal (#402)

theories/lang/cpp/logic/heap_pred.v
@@ -10,37 +10,10 @@ Require Import Coq.Strings.String.
 
 From iris.bi Require Export monpred.
 
-From bedrock.lang.cpp Require Import semantics logic.pred ast.
+From bedrock.lang.cpp Require Import
+     semantics logic.pred logic.path_pred ast.
 
 Local Open Scope string_scope.
-
-(* representations are predicates over a location, they should be used to
- * assert properties of the heap
- *)
-Global Instance val_inhabited : Inhabited val.
-Proof. constructor. apply (Vint 0). Qed.
-Global Instance ptr_inhabited : Inhabited ptr.
-Proof. constructor. apply nullptr. Qed.
-
-Local Instance ptr_rel : SqSubsetEq ptr.
-Proof.
-  unfold SqSubsetEq.
-  unfold relation.
-  apply eq.
-Defined.
-
-Local Instance ptr_rel_preorder : PreOrder (⊑@{ptr}).
-Proof.
-  unfold sqsubseteq. unfold ptr_rel.
-  apply base.PreOrder_instance_0.
-Qed.
-
-Canonical Structure ptr_bi_index : biIndex :=
-  BiIndex ptr ptr_inhabited ptr_rel ptr_rel_preorder.
-
-Definition Rep Σ := (monPred ptr_bi_index (mpredI Σ)).
-Definition RepI Σ := (monPredI ptr_bi_index (mpredI Σ)).
-Definition RepSI Σ := (monPredSI ptr_bi_index (mpredSI Σ)).
 
 Lemma monPred_at_persistent_inv {V bi} (P : monPred V bi) :
   (∀ i, Persistent (P i)) → Persistent P.
@@ -50,387 +23,225 @@ Lemma monPred_at_timeless_inv {V sbi} (P : monPredSI V sbi) :
   (∀ i, Timeless (P i)) → Timeless P.
 Proof. intros HP. constructor=> i. MonPred.unseal. apply HP. Qed.
 
-Lemma Rep_lequiv {Σ} : forall (P Q : Rep Σ),
-    (forall p, P p -|- Q p) ->
-    P -|- Q.
-Proof.
-  intros. split; constructor; apply H.
-Qed.
-
-
-(* locations are computations that produce an address.
- * - note(gmm): they are always computable from the program except.
- *)
-Definition Loc : Type := option ptr.
-
-Definition Offset : Type := option (ptr -> option ptr).
-
-Section with_Σ.
-Context {Σ : gFunctors}.
-
-Local Notation mpred := (mpred Σ) (only parsing).
-Local Notation Rep := (Rep Σ) (only parsing).
-
-Local Ltac solve_Rep_persistent X :=
-  intros;
-  rewrite X;
-  constructor; apply monPred_at_persistent_inv;
-  apply _.
-Local Ltac solve_Loc_persistent X :=
-  intros;
-  rewrite X;
-  constructor; apply monPred_at_persistent_inv;
-  apply _.
-Local Ltac solve_Offset_persistent X :=
-  intros;
-  rewrite X;
-  constructor; apply monPred_at_persistent_inv;
-  constructor; apply monPred_at_persistent_inv;
-  apply _.
-
-Local Ltac solve_Rep_timeless X :=
-  intros;
-  rewrite X;
-  constructor; apply monPred_at_timeless_inv;
-  apply _.
-Local Ltac solve_Loc_timeless X :=
-  intros;
-  rewrite X;
-  constructor; apply monPred_at_timeless_inv;
-  apply _.
-Local Ltac solve_Offset_timeless X :=
-  intros;
-  rewrite X;
-  constructor; apply monPred_at_timeless_inv;
-  constructor; apply monPred_at_timeless_inv;
-  apply _.
-
-Definition as_Rep (P : ptr -> mpred) : Rep := MonPred P _.
-
-Lemma Rep_equiv_ext_equiv : forall P Q : Rep,
-    (forall x, P x -|- Q x) ->
-    P -|- Q.
-Proof.
-  split; red; simpl; eapply H.
-Qed.
-
-Definition LocEq (l1 l2 : Loc) : Prop :=
-  l1 = l2.
-
-(* absolute locations *)
-Definition _eq_def (p : ptr) : Loc :=
-  Some p.
-Definition _eq_aux : seal (@_eq_def). by eexists. Qed.
-Definition _eq := _eq_aux.(unseal).
-Definition _eq_eq : @_eq = _ := _eq_aux.(seal_eq).
-
-
-Definition _eqv (a : val) : Loc :=
-  match a with
-  | Vptr p => _eq p
-  | _ => None
-  end.
-
-Lemma _eqv_eq : forall p, _eqv (Vptr p) = _eq p.
-Proof. reflexivity. Qed.
-
-(* val -> ptr *)
-Definition this_addr (r : region) (p : ptr) : mpred :=
-  local_addr r "#this" p.
-
-(* val -> ptr *)
-Definition result_addr (r : region) (p : ptr) : mpred :=
-  local_addr r "#result" p.
-
-(* ^ these two could be duplicable because regions don't need to be
- * reused. the reason that local variables need to be tracked is that
- * they could go out of scope.
- * - an alternative, and (sound) solution is to generate a fresh region
- *   each time that we create a new scope. To do this, we need to track in
- *   the AST the debruijn index of the binder.
- * - yet another alternative is to inline regions explicitly into the WP.
- *   essentially region := list (list (string * ptr)). this essentially makes
- *   _local persistent.
- *)
-
-Definition _global_def (resolve : genv) (x : obj_name) : Loc :=
-  match glob_addr resolve x with
-  | None => None
-  | Some p => Some p
-  end.
-Definition _global_aux : seal (@_global_def). by eexists. Qed.
-Definition _global := _global_aux.(unseal).
-Definition _global_eq : @_global = _ := _global_aux.(seal_eq).
-
-(* offsets *)
-Definition _field_def (resolve: genv) (f : field) : Offset :=
-  match offset_of resolve f.(f_type) f.(f_name) with
-  | Some o => Some (fun p => Some (offset_ptr_ o p))
-  | _ => None
-  end.
-Definition _field_aux : seal (@_field_def). Proof using. by eexists. Qed.
-Definition _field := _field_aux.(unseal).
-Definition _field_eq : @_field = _ := _field_aux.(seal_eq).
-
-Definition _sub_def (resolve:genv) (t : type) (i : Z) : Offset :=
-  match size_of resolve t with
-  | Some n => Some (fun p => Some (offset_ptr_ (i * Z.of_N n) p))
-  | _ => None
-  end.
-Definition _sub_aux : seal (@_sub_def). by eexists. Qed.
-Definition _sub := _sub_aux.(unseal).
-Definition _sub_eq : @_sub = _ := _sub_aux.(seal_eq).
-
-
-(* this represents static_cast *)
-Definition _super_def (resolve:genv) (sub super : globname) : Offset :=
-  match parent_offset resolve sub super with
-  | Some o => Some (fun p => Some (offset_ptr_ o p))
-  | _ => None
-  end.
-Definition _super_aux : seal (@_super_def). by eexists. Qed.
-Definition _super := _super_aux.(unseal).
-Definition _super_eq : @_super = _ := _super_aux.(seal_eq).
-
-Definition _id_def : Offset := Some (fun x => Some x).
-Definition _id_aux : seal (@_id_def). by eexists. Qed.
-Definition _id := _id_aux.(unseal).
-Definition _id_eq : @_id = _ := _id_aux.(seal_eq).
-
-Definition _dot_def (o1 o2 : Offset) : Offset :=
-  match o1 , o2 with
-  | Some o1 , Some o2 => Some (fun x => match o1 x with
-                                    | None => None
-                                    | Some p => o2 p
-                                    end)
-  | _ , _ => None
-  end.
-Definition _dot_aux : seal (@_dot_def). by eexists. Qed.
-Definition _dot := _dot_aux.(unseal).
-Definition _dot_eq : @_dot = _ := _dot_aux.(seal_eq).
-
-Definition _offsetL_def (o : Offset) (l : Loc) : Loc :=
-  match o , l with
-  | Some o , Some l => match o l with
-                      | None => None
-                      | Some p => Some p
-                      end
-  | _ , _ => None
-  end.
-Definition _offsetL_aux : seal (@_offsetL_def). by eexists. Qed.
-Definition _offsetL := _offsetL_aux.(unseal).
-Definition _offsetL_eq : @_offsetL = _ := _offsetL_aux.(seal_eq).
-
-
-
-Definition _offsetR_def (o : Offset) (r : Rep) : Rep :=
-  as_Rep (fun a => match o with
-                | Some o => match o a with
-                           | None => lfalse
-                           | Some p => r p
-                           end
-                | None => lfalse
-                end).
-Definition _offsetR_aux : seal (@_offsetR_def). by eexists. Qed.
-Definition _offsetR := _offsetR_aux.(unseal).
-Definition _offsetR_eq : @_offsetR = _ := _offsetR_aux.(seal_eq).
-
-Global Instance _offsetR_persistent o r :
-  Persistent r -> Persistent (_offsetR o r).
-Proof. solve_Rep_persistent _offsetR_eq. Qed.
-Global Instance Proper__offsetR_entails
-  : Proper (eq ==> lentails ==> lentails) _offsetR.
-Proof.
-  rewrite _offsetR_eq. unfold _offsetR_def.
-  constructor. simpl. intros.
-  subst. destruct y; auto. destruct (o i); auto. apply H0.
-Qed.
-
-Global Instance Proper__offsetR_equiv
-  : Proper (eq ==> lequiv ==> lequiv) _offsetR.
-Proof.
-  rewrite _offsetR_eq.
-  intros ?? H1 ?? H2.
-  constructor. simpl.
-  intros. subst. split'; destruct y; try rewrite H2; eauto.
-  all: destruct (o i); eauto; rewrite H2; reflexivity.
-Qed.
-
-
-Definition addr_of_def (a : Loc) (b : ptr) : mpred :=
-  [| a = Some b |].
-Definition addr_of_aux : seal (@addr_of_def). by eexists. Qed.
-Definition addr_of := addr_of_aux.(unseal).
-Definition addr_of_eq : @addr_of = _ := addr_of_aux.(seal_eq).
-Arguments addr_of : simpl never.
-Notation "a &~ b" := (addr_of a b) (at level 30, no associativity).
-
-Global Instance addr_of_persistent : Persistent (addr_of o l).
-Proof. rewrite addr_of_eq. apply _. Qed.
-
-Definition _at_def (base : Loc) (P : Rep) : mpred :=
-  Exists a, base &~ a ** P a.
-Definition _at_aux : seal (@_at_def). by eexists. Qed.
-Definition _at := _at_aux.(unseal).
-Definition _at_eq : @_at = _ := _at_aux.(seal_eq).
-
-Global Instance _at_persistent : Persistent P -> Persistent (_at base P).
-Proof. rewrite _at_eq. apply _. Qed.
-
-Global Instance Proper__at_entails
-  : Proper (eq ==> lentails ==> lentails) _at.
-Proof.
-  rewrite _at_eq. unfold _at_def. red. red. red.
-  intros. simpl in *. subst. setoid_rewrite H0.
-  reflexivity.
-Qed.
-
-Global Instance Proper__at_lequiv
-  : Proper (eq ==> lequiv ==> lequiv) _at.
-Proof.
-  intros x y H1 ?? H2.
-  rewrite _at_eq /_at_def. subst.
-  setoid_rewrite H2.
-  reflexivity.
-Qed.
-
-
-(** Values
- * These `Rep` predicates wrap `ptsto` facts
- *)
-(* todo(gmm): make opaque *)
-Definition pureR (P : mpred) : Rep :=
-  as_Rep (fun _ => P).
-
-Global Instance pureR_persistent (P : mpred) :
-  Persistent P -> Persistent (pureR P).
-Proof. intros. apply monPred_at_persistent_inv. apply  _. Qed.
-
-(* this is the primitive *)
-Definition primR_def {resolve:genv} (ty : type) q (v : val) : Rep :=
-  as_Rep (fun addr => @tptsto _ resolve ty q (Vptr addr) v ** [| has_type v (drop_qualifiers ty) |]).
-Definition primR_aux : seal (@primR_def). by eexists. Qed.
-Definition primR := primR_aux.(unseal).
-Definition primR_eq : @primR = _ := primR_aux.(seal_eq).
-Arguments primR {resolve} ty q v : rename.
-
-Global Instance primR_timeless resolve ty q p : Timeless (primR (resolve:=resolve) ty q p).
-Proof. solve_Rep_timeless primR_eq. Qed.
-
-Global Instance Proper_primR_entails
-: Proper (genv_leq ==> (=) ==> (=) ==> (=) ==> lentails) (@primR).
-Proof.
-  do 5 red; intros; subst.
-  rewrite primR_eq /primR_def. constructor; simpl.
-  intros. setoid_rewrite H. reflexivity.
-Qed.
-Global Instance Proper_primR_equiv
-: Proper (genv_eq ==> (=) ==> (=) ==> (=) ==> lequiv) (@primR).
-Proof.
-  do 5 red; intros; subst.
-  rewrite primR_eq /primR_def. constructor; simpl.
-  intros. setoid_rewrite H. reflexivity.
-Qed.
-
-Definition uninit_def {resolve:genv} (ty : type) q : Rep :=
-  as_Rep (fun addr => Exists v : val, (primR (resolve:=resolve) ty q v) addr ).
-(* todo(gmm): this isn't exactly correct, I need a Vundef *)
-Definition uninit_aux : seal (@uninit_def). by eexists. Qed.
-Definition uninitR := uninit_aux.(unseal).
-Definition uninit_eq : @uninitR = _ := uninit_aux.(seal_eq).
-Arguments uninitR {resolve} ty q : rename.
-
-Global Instance uninit_timeless resolve ty q : Timeless (uninitR (resolve:=resolve) ty q).
-Proof. solve_Rep_timeless uninit_eq. Qed.
-
-(* this means "anything, including uninitialized" *)
-Definition anyR_def {resolve} (ty : type) q : Rep :=
-  as_Rep (fun addr => (Exists v, (primR (resolve:=resolve) ty q v) addr) \\//
-       (uninitR (resolve:=resolve) ty q) addr).
-Definition anyR_aux : seal (@anyR_def). by eexists. Qed.
-Definition anyR := anyR_aux.(unseal).
-Definition anyR_eq : @anyR = _ := anyR_aux.(seal_eq).
-Arguments anyR {resolve} ty q : rename.
-
-Global Instance anyR_timeless resolve ty q : Timeless (anyR (resolve:=resolve) ty q).
-Proof. solve_Rep_timeless anyR_eq. Qed.
-
-Definition tref_def (ty : type) (p : ptr) : Rep :=
-  as_Rep (fun addr => [| addr = p |]).
-Definition tref_aux : seal (@tref_def). by eexists. Qed.
-Definition refR := tref_aux.(unseal).
-Definition tref_eq : @refR = _ := tref_aux.(seal_eq).
-
-Global Instance tref_timeless ty p : Timeless (refR ty p).
-Proof. solve_Rep_timeless tref_eq. Qed.
-
-
-(********************* DERIVED CONCEPTS ****************************)
-
-Definition is_null_def : Rep :=
-  as_Rep (fun addr => [| addr = nullptr |]).
-Definition is_null_aux : seal (@is_null_def). by eexists. Qed.
-Definition is_null := is_null_aux.(unseal).
-Definition is_null_eq : @is_null = _ := is_null_aux.(seal_eq).
-
-Global Instance is_null_persistent : Persistent (is_null).
-Proof. solve_Rep_persistent is_null_eq. Qed.
-
-Definition is_nonnull_def : Rep :=
-  as_Rep (fun addr => [| addr <> nullptr |]).
-Definition is_nonnull_aux : seal (@is_nonnull_def). by eexists. Qed.
-Definition is_nonnull := is_nonnull_aux.(unseal).
-Definition is_nonnull_eq : @is_nonnull = _ := is_nonnull_aux.(seal_eq).
-
-Global Instance is_nonnull_persistent : Persistent (is_nonnull).
-Proof. solve_Rep_persistent is_nonnull_eq. Qed.
-
-Definition tlocal_at_def (r : region) (l : ident) (p : ptr) (v : Rep) : mpred :=
-  local_addr r l p ** _at (_eq p) v.
-Definition tlocal_at_aux : seal (@tlocal_at_def). by eexists. Qed.
-Definition tlocal_at := tlocal_at_aux.(unseal).
-Definition tlocal_at_eq : @tlocal_at = _ := tlocal_at_aux.(seal_eq).
-
-Definition tlocal_def (r : region) (x : ident) (v : Rep) : mpred :=
-  Exists a, tlocal_at r x a v.
-Definition tlocal_aux : seal (@tlocal_def). by eexists. Qed.
-Definition tlocal := tlocal_aux.(unseal).
-Definition tlocal_eq : @tlocal = _ := tlocal_aux.(seal_eq).
-
-(* this is for `Indirect` field references *)
-Fixpoint path_to_Offset (resolve:genv) (from : globname) (final : ident)
-         (ls : list (ident * globname))
-: Offset :=
-  match ls with
-  | nil => @_field resolve {| f_type := from ; f_name := final |}
-  | cons (i,c) ls =>
-    _dot (@_field resolve {| f_type := from ; f_name := i |}) (path_to_Offset resolve c final ls)
-  end.
-
-Definition offset_for (resolve:genv) (cls : globname) (f : FieldOrBase) : Offset :=
-  match f with
-  | Base parent => _super resolve cls parent
-  | Field i => _field resolve {| f_type := cls ; f_name := i |}
-  | Indirect ls final =>
-    path_to_Offset resolve cls final ls
-  | This => _id
-  end.
-
-Global Opaque (* _local _global  *)_at _sub _field _offsetR _offsetL _dot primR (* tint tuint ptrR is_null is_nonnull *) addr_of.
-
-End with_Σ.
-
-Arguments addr_of : simpl never.
-Notation "a &~ b" := (addr_of a b) (at level 30, no associativity).
-Coercion pureR : mpred >-> Rep.
-
-Global Opaque this_addr result_addr.
-
-Arguments anyR {Σ resolve} ty q : rename.
-Arguments uninitR {Σ resolve} ty q : rename.
-Arguments primR {Σ resolve} ty q v : rename.
-Arguments refR {Σ} ty v : rename.
-Arguments _super {resolve} _ _ : rename.
-Arguments _field {resolve} _ : rename.
-Arguments _sub {resolve} _ : rename.
-Arguments _global {resolve} _ : rename.
+
+Section with_cpp.
+  Context `{Σ : cpp_logic}.
+
+  (* representations are predicates over a location, they should be used to
+   * assert properties of the heap
+   *)
+  Global Instance val_inhabited : Inhabited val.
+  Proof. constructor. apply (Vint 0). Qed.
+  Global Instance ptr_inhabited : Inhabited ptr.
+  Proof. constructor. apply nullptr. Qed.
+
+  Local Instance ptr_rel : SqSubsetEq ptr.
+  Proof.
+    unfold SqSubsetEq.
+    unfold relation.
+    apply eq.
+  Defined.
+
+  Local Instance ptr_rel_preorder : PreOrder (⊑@{ptr}).
+  Proof.
+    unfold sqsubseteq. unfold ptr_rel.
+    apply base.PreOrder_instance_0.
+  Qed.
+
+  Canonical Structure ptr_bi_index : biIndex :=
+    BiIndex ptr ptr_inhabited ptr_rel ptr_rel_preorder.
+
+  Definition Rep := monPred ptr_bi_index mpredI.
+  Definition RepI := monPredI ptr_bi_index mpredI.
+  Definition RepSI := monPredSI ptr_bi_index mpredSI.
+
+
+  Lemma Rep_lequiv : forall (P Q : Rep),
+      (forall p, P p -|- Q p) ->
+      P -|- Q.
+  Proof. intros. split'; constructor; intro; rewrite H; reflexivity. Qed.
+
+  Local Ltac solve_Rep_persistent X :=
+    intros;
+    rewrite X;
+    constructor; apply monPred_at_persistent_inv;
+    apply _.
+
+  Local Ltac solve_Rep_timeless X :=
+    intros;
+    rewrite X;
+    constructor; apply monPred_at_timeless_inv;
+    apply _.
+
+  Definition as_Rep (P : ptr -> mpred) : Rep := MonPred P _.
+
+  Lemma Rep_equiv_ext_equiv : forall P Q : Rep,
+      (forall x, P x -|- Q x) ->
+      P -|- Q.
+  Proof.
+    split; red; simpl; eapply H.
+  Qed.
+
+  Definition _offsetR_def (o : Offset) (r : Rep) : Rep :=
+    as_Rep (fun a => match o with
+                  | Some o => match o a with
+                             | None => lfalse
+                             | Some p => r p
+                             end
+                  | None => lfalse
+                  end).
+  Definition _offsetR_aux : seal (@_offsetR_def). by eexists. Qed.
+  Definition _offsetR := _offsetR_aux.(unseal).
+  Definition _offsetR_eq : @_offsetR = _ := _offsetR_aux.(seal_eq).
+
+  Global Instance _offsetR_persistent o r :
+    Persistent r -> Persistent (_offsetR o r).
+  Proof. solve_Rep_persistent _offsetR_eq. Qed.
+  Global Instance Proper__offsetR_entails
+    : Proper (eq ==> lentails ==> lentails) _offsetR.
+  Proof.
+    rewrite _offsetR_eq. unfold _offsetR_def.
+    constructor. simpl. intros.
+    subst. destruct y; auto. destruct (o i); auto. apply H0.
+  Qed.
+
+  Global Instance Proper__offsetR_equiv
+    : Proper (eq ==> lequiv ==> lequiv) _offsetR.
+  Proof.
+    rewrite _offsetR_eq.
+    intros ?? H1 ?? H2.
+    constructor. simpl.
+    intros. subst. split'; destruct y; try rewrite H2; eauto.
+    all: destruct (o i); eauto; rewrite H2; reflexivity.
+  Qed.
+
+  Definition _at_def (base : Loc) (P : Rep) : mpred :=
+    Exists a, base &~ a ** P a.
+  Definition _at_aux : seal (@_at_def). by eexists. Qed.
+  Definition _at := _at_aux.(unseal).
+  Definition _at_eq : @_at = _ := _at_aux.(seal_eq).
+
+  Global Instance _at_persistent : Persistent P -> Persistent (_at base P).
+  Proof. rewrite _at_eq. apply _. Qed.
+
+  Global Instance Proper__at_entails
+    : Proper (eq ==> lentails ==> lentails) _at.
+  Proof.
+    rewrite _at_eq. unfold _at_def. red. red. red.
+    intros. simpl in *. subst. setoid_rewrite H0.
+    reflexivity.
+  Qed.
+
+  Global Instance Proper__at_lequiv
+    : Proper (eq ==> lequiv ==> lequiv) _at.
+  Proof.
+    intros x y H1 ?? H2.
+    rewrite _at_eq /_at_def. subst.
+    setoid_rewrite H2.
+    reflexivity.
+  Qed.
+
+  (** Values
+   * These `Rep` predicates wrap `ptsto` facts
+   *)
+  (* todo(gmm): make opaque *)
+  Definition pureR (P : mpred) : Rep :=
+    as_Rep (fun _ => P).
+
+  Global Instance pureR_persistent (P : mpred) :
+    Persistent P -> Persistent (pureR P).
+  Proof. intros. apply monPred_at_persistent_inv. apply  _. Qed.
+
+  (* this is the primitive *)
+  Definition primR_def {resolve:genv} (ty : type) q (v : val) : Rep :=
+    as_Rep (fun addr => @tptsto _ _ resolve ty q addr v ** [| has_type v (drop_qualifiers ty) |]).
+  Definition primR_aux : seal (@primR_def). by eexists. Qed.
+  Definition primR := primR_aux.(unseal).
+  Definition primR_eq : @primR = _ := primR_aux.(seal_eq).
+  Arguments primR {resolve} ty q v : rename.
+
+  Global Instance primR_timeless resolve ty q p : Timeless (primR (resolve:=resolve) ty q p).
+  Proof. solve_Rep_timeless primR_eq. Qed.
+
+  Global Instance Proper_primR_entails
+    : Proper (genv_leq ==> (=) ==> (=) ==> (=) ==> lentails) (@primR).
+  Proof.
+    do 5 red; intros; subst.
+    rewrite primR_eq /primR_def. constructor; simpl.
+    intros. setoid_rewrite H. reflexivity.
+  Qed.
+  Global Instance Proper_primR_equiv
+    : Proper (genv_eq ==> (=) ==> (=) ==> (=) ==> lequiv) (@primR).
+  Proof.
+    do 5 red; intros; subst.
+    rewrite primR_eq /primR_def. constructor; simpl.
+    intros. setoid_rewrite H. reflexivity.
+  Qed.
+
+  Definition uninit_def {resolve:genv} (ty : type) q : Rep :=
+    as_Rep (fun addr => Exists v : val, (primR (resolve:=resolve) ty q v) addr ).
+  (* todo(gmm): this isn't exactly correct, I need a Vundef *)
+  Definition uninit_aux : seal (@uninit_def). by eexists. Qed.
+  Definition uninitR := uninit_aux.(unseal).
+  Definition uninit_eq : @uninitR = _ := uninit_aux.(seal_eq).
+  Arguments uninitR {resolve} ty q : rename.
+
+  Global Instance uninit_timeless resolve ty q : Timeless (uninitR (resolve:=resolve) ty q).
+  Proof. solve_Rep_timeless uninit_eq. Qed.
+
+  (* this means "anything, including uninitialized" *)
+  Definition anyR_def {resolve} (ty : type) q : Rep :=
+    as_Rep (fun addr => (Exists v, (primR (resolve:=resolve) ty q v) addr) \\//
+                                                                        (uninitR (resolve:=resolve) ty q) addr).
+  Definition anyR_aux : seal (@anyR_def). by eexists. Qed.
+  Definition anyR := anyR_aux.(unseal).
+  Definition anyR_eq : @anyR = _ := anyR_aux.(seal_eq).
+  Arguments anyR {resolve} ty q : rename.
+
+  Global Instance anyR_timeless resolve ty q : Timeless (anyR (resolve:=resolve) ty q).
+  Proof. solve_Rep_timeless anyR_eq. Qed.
+
+  Definition tref_def (ty : type) (p : ptr) : Rep :=
+    as_Rep (fun addr => [| addr = p |]).
+  Definition tref_aux : seal (@tref_def). by eexists. Qed.
+  Definition refR := tref_aux.(unseal).
+  Definition tref_eq : @refR = _ := tref_aux.(seal_eq).
+
+  Global Instance tref_timeless ty p : Timeless (refR ty p).
+  Proof. solve_Rep_timeless tref_eq. Qed.
+
+
+  (********************* DERIVED CONCEPTS ****************************)
+
+  Definition is_null_def : Rep :=
+    as_Rep (fun addr => [| addr = nullptr |]).
+  Definition is_null_aux : seal (@is_null_def). by eexists. Qed.
+  Definition is_null := is_null_aux.(unseal).
+  Definition is_null_eq : @is_null = _ := is_null_aux.(seal_eq).
+
+  Global Instance is_null_persistent : Persistent (is_null).
+  Proof. solve_Rep_persistent is_null_eq. Qed.
+
+  Definition is_nonnull_def : Rep :=
+    as_Rep (fun addr => [| addr <> nullptr |]).
+  Definition is_nonnull_aux : seal (@is_nonnull_def). by eexists. Qed.
+  Definition is_nonnull := is_nonnull_aux.(unseal).
+  Definition is_nonnull_eq : @is_nonnull = _ := is_nonnull_aux.(seal_eq).
+
+  Global Instance is_nonnull_persistent : Persistent (is_nonnull).
+  Proof. solve_Rep_persistent is_nonnull_eq. Qed.
+
+  Definition tlocal_at_def (r : region) (l : ident) (p : ptr) (v : Rep) : mpred :=
+    local_addr r l p ** _at (_eq p) v.
+  Definition tlocal_at_aux : seal (@tlocal_at_def). by eexists. Qed.
+  Definition tlocal_at := tlocal_at_aux.(unseal).
+  Definition tlocal_at_eq : @tlocal_at = _ := tlocal_at_aux.(seal_eq).
+
+End with_cpp.
+
+Global Opaque _at _offsetR primR.
+
+Arguments anyR {_ Σ resolve} ty q : rename.
+Arguments uninitR {_ Σ resolve} ty q : rename.
+Arguments primR {_ Σ resolve} ty q v : rename.
+Arguments refR {_ Σ} ty v : rename.
