theories/lang/cpp/logic/wp.v
@@ -10,18 +10,13 @@
 Require Import Coq.Lists.List.
 Require Import Coq.Strings.String.
 
+Require Import iris.bi.monpred.
 From iris.proofmode Require Import tactics.
 
 From bedrock.lang.cpp Require Import
      ast semantics logic.pred.
 
 Set Primitive Projections.
-
-(* expression continuations
- * - in full C++, this includes exceptions, but our current semantics
- *   doesn't treat those.
- *)
-Definition epred Σ := mpred Σ.
 
 (* this applies `wp` across a list
  *
@@ -39,251 +34,241 @@ Section wps.
     end.
 End wps.
 
-Definition FreeTemps Σ := mpred Σ.
-(** Expressions *)
-Section with_Σ.
-Context {Σ : gFunctors}.
 
-Notation mpred := (mpred Σ) (only parsing).
-Notation FreeTemps := (FreeTemps Σ) (only parsing).
-Notation epred := (epred Σ) (only parsing).
+Section with_cpp.
+  Context `{Σ : cpp_logic thread_info}.
 
-(* [SP] denotes the sequence point for an expression *)
-Definition SP (Q : val -> mpred) (v : val) (free : FreeTemps) : mpred :=
-  free ** Q v.
+  (* expression continuations
+   * - in full C++, this includes exceptions, but our current semantics
+   *   doesn't treat those.
+   *)
+  Definition epred := mpred.
 
-(* evaluate an expression as an lvalue *)
-Parameter wp_lval
-  : forall {resolve:genv}, thread_info -> region ->
-    Expr ->
-    (val -> FreeTemps -> epred) -> (* result -> free -> post *)
-    mpred. (* pre-condition *)
+  Definition FreeTemps := mpred.
 
-Axiom Proper_wp_lval :
-    Proper (genv_leq ==> eq ==> eq ==> eq ==> (pointwise_relation _ (pointwise_relation _ lentails)) ==> lentails)
+  (* [SP] denotes the sequence point for an expression *)
+  Definition SP (Q : val -> mpred) (v : val) (free : FreeTemps) : mpred :=
+    free ** Q v.
+
+  (* evaluate an expression as an lvalue *)
+  Parameter wp_lval
+    : forall {resolve:genv}, thread_info -> region ->
+        Expr ->
+        (val -> FreeTemps -> epred) -> (* result -> free -> post *)
+        mpred. (* pre-condition *)
+
+  Axiom Proper_wp_lval :
+    Proper (genv_leq ==> eq ==> eq ==> eq ==>
+            pointwise_relation _ (pointwise_relation _ lentails) ==> lentails)
            (@wp_lval).
-Global Existing Instance Proper_wp_lval.
+  Global Existing Instance Proper_wp_lval.
 
-(* evaluate an expression as an prvalue *)
-Parameter wp_prval
-  : forall {resolve:genv}, thread_info -> region ->
-    Expr ->
-    (val -> FreeTemps -> epred) -> (* result -> free -> post *)
-    mpred. (* pre-condition *)
+  (* evaluate an expression as an prvalue *)
+  Parameter wp_prval
+    : forall {resolve:genv}, thread_info -> region ->
+        Expr ->
+        (val -> FreeTemps -> epred) -> (* result -> free -> post *)
+        mpred. (* pre-condition *)
 
-Axiom Proper_wp_prval :
-    Proper (genv_leq ==> eq ==> eq ==> eq ==> (pointwise_relation _ (pointwise_relation _ lentails)) ==> lentails)
+  Axiom Proper_wp_prval :
+    Proper (genv_leq ==> eq ==> eq ==> eq ==>
+            pointwise_relation _ (pointwise_relation _ lentails) ==> lentails)
            (@wp_prval).
-Global Existing Instance Proper_wp_prval.
+  Global Existing Instance Proper_wp_prval.
 
-(* evaluate an initializing expression
- * - the [val] is the location of the value that is being initialized
- * - the expression denotes a prvalue with a "result object" (see
- *    https://en.cppreference.com/w/cpp/language/value_category)
- *)
-Parameter wp_init
-  : forall {resolve:genv}, thread_info -> region ->
-    type -> val -> Expr ->
-    (FreeTemps -> epred) -> (* free -> post *)
-    mpred. (* pre-condition *)
-Axiom Proper_wp_init :
-    Proper (genv_leq ==> eq ==> eq ==> eq ==> eq ==> eq ==> pointwise_relation _ lentails ==> lentails)
+  (* evaluate an initializing expression
+   * - the [val] is the location of the value that is being initialized
+   * - the expression denotes a prvalue with a "result object" (see
+   *    https://en.cppreference.com/w/cpp/language/value_category)
+   *)
+  Parameter wp_init
+    : forall {resolve:genv}, thread_info -> region ->
+                        type -> val -> Expr ->
+                        (FreeTemps -> epred) -> (* free -> post *)
+                        mpred. (* pre-condition *)
+  Axiom Proper_wp_init :
+    Proper (genv_leq ==> eq ==> eq ==> eq ==> eq ==> eq ==>
+            pointwise_relation _ lentails ==> lentails)
            (@wp_init).
-Global Existing Instance Proper_wp_init.
+  Global Existing Instance Proper_wp_init.
 
 
-(* evaluate an expression as an xvalue *)
-Parameter wp_xval
-  : forall {resolve:genv}, thread_info -> region ->
-    Expr ->
-    (val -> FreeTemps -> epred) -> (* result -> free -> post *)
-    mpred. (* pre-condition *)
+  (* evaluate an expression as an xvalue *)
+  Parameter wp_xval
+    : forall {resolve:genv}, thread_info -> region ->
+                        Expr ->
+                        (val -> FreeTemps -> epred) -> (* result -> free -> post *)
+                        mpred. (* pre-condition *)
 
-Axiom Proper_wp_xval :
-    Proper (genv_leq ==> eq ==> eq ==> eq ==> (pointwise_relation _ (pointwise_relation _ lentails)) ==> lentails)
+  Axiom Proper_wp_xval :
+    Proper (genv_leq ==> eq ==> eq ==> eq ==>
+            pointwise_relation _ (pointwise_relation _ lentails) ==> lentails)
            (@wp_xval).
-Global Existing Instance Proper_wp_xval.
+  Global Existing Instance Proper_wp_xval.
 
-Definition wp_glval {resolve} (ti : thread_info) (r : region) e Q :=
-  @wp_lval resolve ti r e Q \\//
-  @wp_xval resolve ti r e Q.
-Theorem Proper_wp_glval :
-    Proper (genv_leq ==> eq ==> eq ==> eq ==> (pointwise_relation _ (pointwise_relation _ lentails)) ==> lentails)
+  Definition wp_glval {resolve} ti (r : region) e Q :=
+    @wp_lval resolve ti r e Q \\// @wp_xval resolve ti r e Q.
+  Theorem Proper_wp_glval :
+    Proper (genv_leq ==> eq ==> eq ==> eq ==>
+            pointwise_relation _ (pointwise_relation _ lentails) ==> lentails)
            (@wp_glval).
-Proof.
-  unfold wp_glval; simpl. do 7 red. intros.
-  eapply bi.or_elim; [ rewrite <- bi.or_intro_l | rewrite <- bi.or_intro_r ].
-  eapply Proper_wp_lval; eauto.
-  eapply Proper_wp_xval; eauto.
-Qed.
-Global Existing Instance Proper_wp_glval.
+  Proof.
+    unfold wp_glval; simpl. do 6 red. intros.
+    eapply bi.or_elim; [ rewrite <- bi.or_intro_l | rewrite <- bi.or_intro_r ].
+    eapply Proper_wp_lval; eauto.
+    eapply Proper_wp_xval; eauto.
+  Qed.
+  Global Existing Instance Proper_wp_glval.
 
 
-Definition wp_rval {resolve} (ti : thread_info) (r : region) e Q :=
-  @wp_prval resolve ti r e Q \\//
-  @wp_xval resolve ti r e Q.
-Theorem Proper_wp_rval :
-    Proper (genv_leq ==> eq ==> eq ==> eq ==> (pointwise_relation _ (pointwise_relation _ lentails)) ==> lentails)
+  Definition wp_rval {resolve} ti (r : region) e Q :=
+    @wp_prval resolve ti r e Q \\// @wp_xval resolve ti r e Q.
+  Theorem Proper_wp_rval :
+    Proper (genv_leq ==> eq ==> eq ==> eq ==>
+            pointwise_relation _ (pointwise_relation _ lentails) ==> lentails)
            (@wp_rval).
-Proof.
-  unfold wp_rval; simpl. do 7 red. intros.
-  eapply bi.or_elim; [ rewrite <- bi.or_intro_l | rewrite <- bi.or_intro_r ].
-  eapply Proper_wp_prval; eauto.
-  eapply Proper_wp_xval; eauto.
-Qed.
-Global Existing Instance Proper_wp_rval.
+  Proof.
+    unfold wp_rval; simpl. do 6 red. intros.
+    eapply bi.or_elim; [ rewrite <- bi.or_intro_l | rewrite <- bi.or_intro_r ].
+    eapply Proper_wp_prval; eauto.
+    eapply Proper_wp_xval; eauto.
+  Qed.
+  Global Existing Instance Proper_wp_rval.
 
-Section wpe.
-  Context {resolve:genv}.
-  Variable ti : thread_info.
-  Variable ρ : region.
+  Section wpe.
+    Context {resolve:genv}.
+    Variable (ti : thread_info) (ρ : region).
 
-  Definition wpe (vc : ValCat)
-  : Expr -> (val -> FreeTemps -> mpred) -> mpred :=
-    match vc with
-    | Lvalue => @wp_lval resolve ti ρ
-    | Rvalue => @wp_prval resolve ti ρ
-    | Xvalue => @wp_xval resolve ti ρ
-    end.
+    Definition wpe (vc : ValCat)
+      : Expr -> (val -> FreeTemps -> mpred) -> mpred :=
+      match vc with
+      | Lvalue => @wp_lval resolve ti ρ
+      | Rvalue => @wp_prval resolve ti ρ
+      | Xvalue => @wp_xval resolve ti ρ
+      end.
 
-  Definition wpAny (vce : ValCat * Expr)
-  : (val -> FreeTemps -> mpred) -> mpred :=
-    let '(vc,e) := vce in
-    wpe vc e.
+    Definition wpAny (vce : ValCat * Expr)
+      : (val -> FreeTemps -> mpred) -> mpred :=
+      let '(vc,e) := vce in
+      wpe vc e.
 
-  Definition wpAnys := fun ve Q free => wpAny ve (fun v f => Q v (f ** free)).
-End wpe.
+    Definition wpAnys := fun ve Q free => wpAny ve (fun v f => Q v (f ** free)).
+  End wpe.
 
-(** initializers *)
-Parameter wpi
-  : forall {resolve:genv} (ti : thread_info) (ρ : region)
-      (cls : globname) (this : val) (init : Initializer)
-      (Q : mpred -> mpred), mpred.
+  (** initializers *)
+  Parameter wpi
+    : forall {resolve:genv} (ti : thread_info) (ρ : region)
+        (cls : globname) (this : val) (init : Initializer)
+        (Q : mpred -> mpred), mpred.
 
-(* Axiom Proper_wpi : *)
-(*     Proper (genv_leq ==> eq ==> eq ==> eq ==> eq ==> eq ==> (lentails ==> lentails) ==> lentails) *)
-(*            (@wpi). *)
-(* Global Existing Instance Proper_wp_prval. *)
+  Axiom Proper_wpi :
+    Proper (genv_leq ==> eq ==> eq ==> eq ==> eq ==> eq ==> (lentails ==> lentails) ==> lentails)
+           (@wpi).
+  Global Existing Instance Proper_wp_prval.
 
+  (** destructors *)
+  Parameter wpd
+    : forall {resolve:genv} (ti : thread_info) (ρ : region)
+        (cls : globname) (this : val)
+        (init : FieldOrBase * obj_name)
+        (Q : epred), mpred.
 
-(** destructors *)
-Parameter wpd
-  : forall {resolve:genv} (ti : thread_info) (ρ : region)
-      (cls : globname) (this : val)
-      (init : FieldOrBase * obj_name)
-      (Q : mpred), mpred.
+  (** Statements *)
+  (* continuations
+   * C++ statements can terminate in 4 ways.
+   *
+   * note(gmm): technically, they can also raise exceptions; however,
+   * our current semantics doesn't capture this. if we want to support
+   * exceptions, we should be able to add another case,
+   * `k_throw : val -> mpred`.
+   *)
+  Record Kpreds :=
+    { k_normal   : mpred
+    ; k_return   : option val -> FreeTemps -> mpred
+    ; k_break    : mpred
+    ; k_continue : mpred
+    }.
 
+  Definition void_return (P : mpred) : Kpreds :=
+    {| k_normal := P
+     ; k_return := fun r free => match r with
+                              | None => free ** P
+                              | Some _ => lfalse
+                              end
+     ; k_break := lfalse
+     ; k_continue := lfalse
+    |}.
 
-End with_Σ.
+  Definition val_return (P : val -> mpred) : Kpreds :=
+    {| k_normal := lfalse
+     ; k_return := fun r free => match r with
+                              | None => lfalse
+                              | Some v => free ** P v
+                              end
+     ; k_break := lfalse
+     ; k_continue := lfalse |}.
 
-(** Statements *)
-(* continuations
- * C++ statements can terminate in 4 ways.
- *
- * note(gmm): technically, they can also raise exceptions; however,
- * our current semantics doesn't capture this. if we want to support
- * exceptions, we should be able to add another case,
- * `k_throw : val -> mpred`.
- *)
-Record Kpreds Σ :=
-  { k_normal   : mpred Σ
-  ; k_return   : option val -> FreeTemps Σ -> mpred Σ
-  ; k_break    : mpred Σ
-  ; k_continue : mpred Σ
-  }.
-Arguments k_normal {_}.
-Arguments k_return {_} _ _.
-Arguments k_break {_}.
-Arguments k_continue {_}.
+  Definition Kseq (Q : Kpreds -> mpred) (k : Kpreds) : Kpreds :=
+    {| k_normal   := Q k
+     ; k_return   := k.(k_return)
+     ; k_break    := k.(k_break)
+     ; k_continue := k.(k_continue) |}.
 
-Section with_Σ.
-Context `{Σ : gFunctors}.
+  (* loop with invariant `I` *)
+  Definition Kloop (I : mpred) (Q : Kpreds) : Kpreds :=
+    {| k_break    := Q.(k_normal)
+     ; k_continue := I
+     ; k_return   := Q.(k_return)
+     ; k_normal   := Q.(k_normal) |}.
 
-Notation mpred := (mpred Σ) (only parsing).
-Notation epred := (epred Σ) (only parsing).
-Notation FreeTemps := (FreeTemps Σ) (only parsing).
-Notation Kpreds := (Kpreds Σ) (only parsing).
+  Definition Kat_exit (Q : mpred -> mpred) (k : Kpreds) : Kpreds :=
+    {| k_normal   := Q k.(k_normal)
+     ; k_return v free := Q (k.(k_return) v free)
+     ; k_break    := Q k.(k_break)
+     ; k_continue := Q k.(k_continue) |}.
 
-Definition void_return (P : mpred) : Kpreds :=
-  {| k_normal := P
-   ; k_return := fun r free => match r with
-                            | None => free ** P
-                            | Some _ => lfalse
-                            end
-   ; k_break := lfalse
-   ; k_continue := lfalse
-   |}.
+  Definition Kfree (a : mpred) : Kpreds -> Kpreds :=
+    Kat_exit (fun P => a ** P).
 
-Definition val_return (P : val -> mpred) : Kpreds :=
-  {| k_normal := lfalse
-   ; k_return := fun r free => match r with
-                            | None => lfalse
-                            | Some v => free ** P v
-                            end
-   ; k_break := lfalse
-   ; k_continue := lfalse |}.
+  Global Instance Kpreds_equiv : Equiv Kpreds :=
+    fun (k1 k2 : Kpreds) =>
+      k1.(k_normal) ≡ k2.(k_normal) ∧
+      (∀ v free, k1.(k_return) v free ≡ k2.(k_return) v free) ∧
+      k1.(k_break) ≡ k2.(k_break) ∧
+      k1.(k_continue) ≡ k2.(k_continue).
 
-Definition Kseq (Q : Kpreds -> mpred) (k : Kpreds) : Kpreds :=
-  {| k_normal   := Q k
-   ; k_return   := k.(k_return)
-   ; k_break    := k.(k_break)
-   ; k_continue := k.(k_continue) |}.
+  Lemma Kfree_Kfree : forall k P Q, Kfree P (Kfree Q k) ≡ Kfree (P ** Q) k.
+  Proof.
+    split; [ | split; [ | split ] ]; simpl; intros;
+      eapply bi.equiv_spec; split;
+        try solve [ rewrite bi.sep_assoc; eauto ].
+  Qed.
 
-(* loop with invariant `I` *)
-Definition Kloop (I : mpred) (Q : Kpreds) : Kpreds :=
-  {| k_break    := Q.(k_normal)
-   ; k_continue := I
-   ; k_return   := Q.(k_return)
-   ; k_normal   := Q.(k_normal) |}.
+  Lemma Kfree_emp : forall k, Kfree empSP k ≡ k.
+  Proof.
+    split; [ | split; [ | split ] ]; simpl; intros;
+      eapply bi.equiv_spec; split;
+        try solve [ rewrite bi.emp_sep; eauto ].
+  Qed.
 
-Definition Kat_exit (Q : mpred -> mpred) (k : Kpreds) : Kpreds :=
-  {| k_normal   := Q k.(k_normal)
-   ; k_return v free := Q (k.(k_return) v free)
-   ; k_break    := Q k.(k_break)
-   ; k_continue := Q k.(k_continue) |}.
+  (* evaluate a statement *)
+  Parameter wp
+    : forall {resolve:genv}, thread_info -> region -> Stmt -> Kpreds -> mpred.
 
-Definition Kfree (a : mpred) : Kpreds -> Kpreds :=
-  Kat_exit (fun P => a ** P).
-
-Global Instance Kpreds_equiv : Equiv Kpreds :=
-  fun (k1 k2 : Kpreds) =>
-    k1.(k_normal) ≡ k2.(k_normal) ∧
-    (∀ v free, k1.(k_return) v free ≡ k2.(k_return) v free) ∧
-    k1.(k_break) ≡ k2.(k_break) ∧
-    k1.(k_continue) ≡ k2.(k_continue).
-
-Lemma Kfree_Kfree : forall k P Q, Kfree P (Kfree Q k) ≡ Kfree (P ** Q) k.
-Proof.
-  split; [ | split; [ | split ] ]; simpl; intros;
-    eapply bi.equiv_spec; split;
-      try solve [ rewrite bi.sep_assoc; eauto ].
-Qed.
-
-Lemma Kfree_emp : forall k, Kfree empSP k ≡ k.
-Proof.
-  split; [ | split; [ | split ] ]; simpl; intros;
-    eapply bi.equiv_spec; split;
-      try solve [ rewrite bi.emp_sep; eauto ].
-Qed.
-
-(* evaluate a statement *)
-Parameter wp
-  : forall {resolve:genv}, thread_info -> region -> Stmt -> Kpreds -> mpred.
-
-Axiom Proper_wp :
+  Axiom Proper_wp :
     Proper (genv_leq ==> eq ==> eq ==> eq ==> equiv ==> lentails)
            (@wp).
-Global Existing Instance Proper_wp.
+  Global Existing Instance Proper_wp.
 
-(* this is the *semantic characterization* of a function
- * it really says something about the assembly code
- *
- * [addr] represents the address of the entry point of the code.
- *)
-Parameter fspec
-: forall (addr : val) (ti : thread_info) (ls : list val) (Q : val -> epred), mpred.
-(* ^ todo(gmm): is this correct? *)
+  (* this is the *semantic characterization* of a function
+   * it really says something about the assembly code
+   *
+   * [addr] represents the address of the entry point of the code.
+   *)
+  Parameter fspec
+    : forall (ti : thread_info) (addr : val) (ls : list val) (Q : val -> epred), mpred.
+  (* ^ todo(gmm): is this correct? *)
 
-Axiom Proper_fspec : forall a ti ls,
-    Proper (pointwise_relation _ lentails ==> lentails) (@fspec a ti ls).
-End with_Σ.
+  Axiom Proper_fspec : forall a ls ti,
+      Proper (pointwise_relation _ lentails ==> lentails) (@fspec ti a ls).
+End with_cpp.
