theories/lang/cpp/logic/call.v
@@ -13,23 +13,16 @@ Local Open Scope Z_scope.
 Require Import bedrock.lang.cpp.ast.
 Require Import bedrock.lang.cpp.semantics.
 From bedrock.lang.cpp.logic Require Import
-     pred heap_pred wp destroy intensional.
+     pred path_pred heap_pred wp destroy intensional.
 
 Section with_resolve.
-  Context {Σ:gFunctors} {resolve:genv}.
-  Variable ti : thread_info.
-  Variable ρ : region.
+  Context `{Σ : cpp_logic thread_info} {σ : genv}.
+  Variables (ti : thread_info) (ρ : region).
 
-  Local Notation wp := (wp (Σ:=Σ) (resolve:=resolve) ti ρ).
-  Local Notation wpe := (wpe (Σ:=Σ) (resolve:=resolve) ti ρ).
-  Local Notation wp_lval := (wp_lval (Σ:=Σ) (resolve:=resolve) ti ρ).
-  Local Notation wp_rval := (wp_rval (Σ:=Σ) (resolve:=resolve) ti ρ).
-  Local Notation wp_prval := (wp_prval (Σ:=Σ) (resolve:=resolve) ti ρ).
-  Local Notation wp_xval := (wp_xval (Σ:=Σ) (resolve:=resolve) ti ρ).
-  Local Notation wp_init := (wp_init (Σ:=Σ) (resolve:=resolve) ti ρ).
-
-  Local Notation mpred := (mpred Σ) (only parsing).
-  Local Notation FreeTemps := (FreeTemps Σ) (only parsing).
+  Local Notation wp_lval := (wp_lval (resolve:=σ) ti ρ).
+  Local Notation wp_prval := (wp_prval (resolve:=σ) ti ρ).
+  Local Notation wp_xval := (wp_xval (resolve:=σ) ti ρ).
+  Local Notation wp_init := (wp_init (resolve:=σ) ti ρ).
 
   Fixpoint wp_args (es : list (ValCat * Expr)) (Q : list val -> FreeTemps -> mpred) : mpred :=
     match es with
@@ -42,10 +35,10 @@ Section with_resolve.
                      wp_args es (fun vs frees => Q (v :: vs) (free ** frees)))
       | Rvalue =>
         if is_aggregate ty then
-          Forall a, _at (_eqv a) (uninitR (resolve:=resolve) (erase_qualifiers ty) 1) -*
+          Forall a, _at (_eqv a) (uninitR (resolve:=σ) (erase_qualifiers ty) 1) -*
           let (e,dt) := destructor_for e in
           wp_init ty a e (fun free => wp_args es (fun vs frees =>
-                                                 Q (a :: vs) (@mdestroy _ resolve ti ty a dt free ** frees)))
+                                                 Q (a :: vs) (mdestroy (σ:=σ) ti ty a dt free ** frees)))
         else
           wp_prval e (fun v free => wp_args es (fun vs frees =>
                                                Q (v :: vs) (free ** frees)))
