theories/lang/cpp/logic/destructors.v
@@ -7,30 +7,18 @@ Require Import Coq.Lists.List.
 
 From bedrock.lang.cpp Require Import ast semantics.
 From bedrock.lang.cpp.logic Require Import
-     pred heap_pred wp.
+     pred path_pred heap_pred wp.
 
 Section with_resolve.
-  Context {Σ:gFunctors} {resolve: genv}.
+  Context `{Σ : cpp_logic thread_info} {σ: genv}.
   Variable ti : thread_info.
   Variable ρ : region.
 
-  Local Notation wp := (wp (Σ:=Σ)  ti ρ).
-  Local Notation wpe := (wpe (Σ:=Σ) ti ρ).
-  Local Notation wp_lval := (wp_lval (Σ:=Σ) ti ρ).
-  Local Notation wp_rval := (wp_rval (Σ:=Σ) ti ρ).
-  Local Notation wp_xval := (wp_xval (Σ:=Σ) ti ρ).
-  Local Notation wpAny := (wpAny (Σ:=Σ) ti ρ).
-  Local Notation wpAnys := (wpAnys (Σ:=Σ) ti ρ).
-  Local Notation fspec := (fspec (Σ:=Σ)).
-
-  Local Notation mpred := (mpred Σ) (only parsing).
-  Local Notation Rep := (Rep Σ) (only parsing).
-
-  Axiom wpd_deinit : forall resolve cls this path dn Q,
-      Exists dp, Exists fp,
-    (@_global resolve dn &~ dp **
-     _offsetL (offset_for resolve cls path) (_eqv this) &~ fp ** ltrue) //\\
-     |> fspec (Vptr dp) ti (this :: nil) (fun _ => Q)
-    |-- @wpd Σ resolve ti ρ cls this (path, dn) Q.
+  Axiom wpd_deinit : forall (cls : globname) (this : val) path dn (Q : epred),
+    Exists dp, Exists fp,
+      (@_global σ dn &~ dp **
+       _offsetL (offset_for σ cls path) (_eqv this) &~ fp ** ltrue) //\\
+      (|> fspec ti (Vptr dp) (this :: nil) (fun _ => Q))
+    |-- wpd (resolve:=σ) ti ρ cls this (path, dn) Q.
 
 End with_resolve.
