theories/lang/cpp/logic/func.v
@@ -15,7 +15,8 @@ From bedrock Require Import ChargeUtil ChargeCompat.
 
 From bedrock.lang.cpp Require Import ast semantics.
 From bedrock.lang.cpp Require Import
-     pred heap_pred wp intensional (* initializers destructors call intensional *).
+     pred path_pred heap_pred
+     wp intensional.
 
 Local Open Scope string_scope.
 
@@ -24,194 +25,187 @@ Local Set Universe Polymorphism.
 
 Module Type Func.
 
-  (* function specifications written in weakest pre-condition style.
-   *
-   * note(gmm): it might be better to make the `list val` into a
-   * `vector val (length fs_arguments)`.
-   *)
-  Record function_spec Σ : Type :=
-  { fs_return : type
-  ; fs_arguments : list type
-  ; fs_spec : thread_info -> list val -> (val -> mpred Σ) -> mpred Σ
-  }.
-  Arguments fs_return {_} _.
-  Arguments fs_arguments {_} _.
-  Arguments fs_spec {_} _.
+  Section with_prop.
+    Context {PROP : bi}.
 
-  Definition type_of_spec `(fs : function_spec Σ) : type :=
+    Record WithEx@{X Z Y} : Type :=
+      { we_ex   : tele@{X}
+      ; we_post : tele_fun@{X Z Y} we_ex (val * PROP) }.
+
+    Definition WithEx_map (f : val -> PROP -> val * PROP) (we : WithEx) : WithEx :=
+      {| we_ex := we.(we_ex)
+       ; we_post := tele_map (fun '(r,Q) => f r Q) we.(we_post) |}.
+
+    Record WithPrePost@{X Z Y} : Type :=
+      { wpp_with : tele@{X}
+      ; wpp_pre  : tele_fun@{X Z Y} wpp_with (list val * PROP)
+      ; wpp_post : tele_fun@{X Z Y} wpp_with WithEx@{X Z Z} }.
+
+    Fixpoint tbi_exist@{X Z Y} {t : tele@{X}} : forall (P : tele_fun@{X Z Y} t PROP), PROP :=
+      match t as t0 return ((t0 -t> PROP) → PROP) with
+      | [tele] => fun x : PROP => x
+      | @TeleS X binder =>
+        fun P : (∀ x : X, binder x -t> PROP) => Exists x : X, tbi_exist (P x)
+      end.
+
+    Fixpoint tbi_forall@{X Z Y} {t : tele@{X}} : forall (P : tele_fun@{X Z Y} t PROP), PROP :=
+      match t as t0 return ((t0 -t> PROP) → PROP) with
+      | [tele] => fun x : PROP => x
+      | @TeleS X binder =>
+        fun P : (∀ x : X, binder x -t> PROP) => Forall x : X, tbi_forall (P x)
+      end.
+
+    Definition WppD@{X Z Y} (wpp : WithPrePost@{X Z Y}) (params : list val) (Q : val -> PROP) : PROP :=
+      tbi_exist@{X Z Y} (tele_bind (TT:=wpp.(wpp_with)) (fun args =>
+         let P := tele_app wpp.(wpp_pre) args in
+         let Q' := tele_app wpp.(wpp_post) args in
+         [| params = fst P |] ** snd P **
+         tbi_forall@{X Z Y} (tele_map (fun '(result,Q') => Q' -* Q result) Q'.(we_post)))).
+
+  End with_prop.
+  Arguments WithPrePost : clear implicits.
+  Arguments Build_WithPrePost _ _ _ : clear implicits.
+  Arguments WithEx : clear implicits.
+  Arguments Build_WithEx _ _ _ : clear implicits.
+
+  Arguments we_ex {PROP} _.
+  Arguments we_post {PROP} _.
+  Arguments wpp_with {_} _.
+  Arguments wpp_pre {_} _.
+  Arguments wpp_post {_} _.
+
+  Global Arguments WppD !_ / .
+
+  Section with_cpp.
+  Context `{Σ : cpp_logic thread_info} {resolve:genv}.
+
+    Record function_spec : Type :=
+      { fs_return : type
+      ; fs_arguments : list type
+      ; fs_spec : thread_info -> list val -> (val -> mpred) -> mpred
+      }.
+  Arguments function_spec : clear implicits.
+  Arguments Build_function_spec : clear implicits.
+
+  (* function specifications written in weakest pre-condition style.
+   *)
+
+  Definition type_of_spec `(fs : function_spec) : type :=
     normalize_type (Tfunction fs.(fs_return) fs.(fs_arguments)).
 
   (* this is the core definition that everything will be based on.
    * it is really an assertion about assembly
    *)
-  Definition cptr_def {Σ} ti (fs : function_spec Σ) : Rep Σ :=
+  Definition cptr_def (fs : function_spec) : Rep :=
     as_Rep (fun p =>
          Forall vs,
          [| List.length vs = List.length fs.(fs_arguments) |] -*
-         Forall Q, fs.(fs_spec) ti vs Q -* fspec (Vptr p) ti vs Q).
+         Forall Q (ti : thread_info), fs.(fs_spec) ti vs Q -* fspec ti (Vptr p) vs Q).
   Definition cptr_aux : seal (@cptr_def). by eexists. Qed.
   Definition cptr := cptr_aux.(unseal).
   Definition cptr_eq : @cptr = _ := cptr_aux.(seal_eq).
-  Arguments cptr {Σ}.
-
-  Record WithEx@{X Z Y} Σ : Type :=
-    { we_ex   : tele@{X}
-    ; we_post : tele_fun@{X Z Y} we_ex (val * mpred Σ) }.
-  Arguments we_ex {Σ} _.
-  Arguments we_post {Σ} _.
-
-  Definition WithEx_map {Σ} (f : val -> mpred Σ -> val * mpred Σ) (we : WithEx Σ) : WithEx Σ :=
-    {| we_ex := we.(we_ex)
-     ; we_post := tele_map (fun '(r,Q) => f r Q) we.(we_post) |}.
-
-  Record WithPrePost@{X Z Y} Σ : Type :=
-    { wpp_with : tele@{X}
-    ; wpp_pre  : tele_fun@{X Z Y} wpp_with (list val * mpred Σ)
-    ; wpp_post : tele_fun@{X Z Y} wpp_with (WithEx@{X Z Z} Σ) }.
-  Arguments wpp_with {_} _.
-  Arguments wpp_pre {_} _.
-  Arguments wpp_post {_} _.
-
-  Section with_Σ.
-  Context {Σ : gFunctors} {resolve:genv}.
-
-  Fixpoint tbi_exist@{X Z Y} {t : tele@{X}} : forall (P : tele_fun@{X Z Y} t (mpred Σ)), mpred Σ :=
-    match t as t0 return ((t0 -t> L.mpred Σ) → L.mpred Σ) with
-    | [tele] => fun x : L.mpred Σ => x
-    | @TeleS X binder =>
-      fun P : (∀ x : X, binder x -t> L.mpred Σ) => Exists x : X, tbi_exist (P x)
-    end.
-
-  Fixpoint tbi_forall@{X Z Y} {t : tele@{X}} : forall (P : tele_fun@{X Z Y} t (mpred Σ)), mpred Σ :=
-    match t as t0 return ((t0 -t> L.mpred Σ) → L.mpred Σ) with
-    | [tele] => fun x : L.mpred Σ => x
-    | @TeleS X binder =>
-      fun P : (∀ x : X, binder x -t> L.mpred Σ) => Forall x : X, tbi_forall (P x)
-    end.
-
-  Definition WppD@{X Z Y} (wpp : WithPrePost@{X Z Y} Σ) (params : list val) (Q : val -> mpred Σ) : mpred Σ.
-  refine (
-    tbi_exist@{X Z Y} (tele_bind (TT:=wpp.(wpp_with)) (fun args =>
-      let P := tele_app wpp.(wpp_pre) args in
-      let Q' := tele_app wpp.(wpp_post) args in
-      [| params = fst P |] ** snd P ** (tbi_forall@{X Z Y} (tele_map (fun '(result,Q') => Q' -* Q result) Q'.(we_post)))))).
-  Defined.
-  Global Arguments WppD !_ / .
-
 
   (* Hoare triple for a function.
    * note(gmm): these should include linkage specifications.
    *)
   Definition TSFunction@{X Z Y} (ret : type) (targs : list type)
-             (PQ : thread_info -> WithPrePost@{X Z Y} Σ)
-  : function_spec Σ :=
+             (PQ : thread_info -> WithPrePost@{X Z Y} mpredI)
+  : function_spec :=
     {| fs_return    := ret
      ; fs_arguments := targs
      ; fs_spec ti   := WppD (PQ ti) |}.
 
-  Definition SFunction@{X Z  Y} (ret : type) (targs : list type)
-             (PQ : WithPrePost@{X Z Y} Σ)
-  : function_spec Σ :=
-    TSFunction ret targs (fun _ => PQ).
 
-  Local Notation uninitR := (@uninitR Σ resolve) (only parsing).
-  Local Notation anyR := (@anyR Σ resolve) (only parsing).
-  Local Notation primR := (@primR Σ resolve) (only parsing).
+  Definition SFunction@{X Z Y} (ret : type) (targs : list type)
+             (PQ : WithPrePost@{X Z Y} mpredI)
+  : function_spec :=
+    {| fs_return    := ret
+     ; fs_arguments := targs
+     ; fs_spec _    := WppD PQ |}.
+
+  Local Notation uninitR := (@uninitR _ Σ resolve) (only parsing).
+  Local Notation anyR := (@anyR _ Σ resolve) (only parsing).
+  Local Notation primR := (@primR _ Σ resolve) (only parsing).
 
   (* Hoare triple for a constructor.
    *)
-  Definition TSConstructor@{X Z Y} (class : globname)
+  Definition SConstructor@{X Z Y} (class : globname)
              (targs : list type)
-             (PQ : thread_info -> ptr -> WithPrePost@{X Z Y} Σ)
-  : function_spec Σ :=
+             (PQ : ptr -> WithPrePost@{X Z Y} mpredI)
+  : function_spec :=
     let map_pre this '(args, P) :=
         (this :: args,
          _at (_eqv this) (uninitR (Tnamed class) 1) ** P) in
     let this_type := Qmut (Tnamed class) in
-    TSFunction (Qmut Tvoid) (Qconst (Tpointer this_type) :: targs)
-               (fun ti =>
-                  {| wpp_with := TeleS (fun this : ptr => (PQ ti this).(wpp_with))
-                   ; wpp_pre this :=
-                       tele_map (map_pre (Vptr this)) (PQ ti this).(wpp_pre)
-                   ; wpp_post this := (PQ ti this).(wpp_post)
-                   |}).
-
-  Definition SConstructor@{X Z Y} (class : globname) (targs : list type)
-             (PQ : ptr -> WithPrePost@{X Z Y} Σ)
-  : function_spec Σ := TSConstructor class targs (fun _ => PQ).
+    SFunction (Qmut Tvoid) (Qconst (Tpointer this_type) :: targs)
+              {| wpp_with := TeleS (fun this : ptr => (PQ this).(wpp_with))
+               ; wpp_pre this :=
+                   tele_map (map_pre (Vptr this)) (PQ this).(wpp_pre)
+               ; wpp_post this := (PQ this).(wpp_post)
+               |}.
 
   (* Hoare triple for a destructor.
    *)
-  Definition TSDestructor@{X Z Y} (class : globname)
-             (PQ : thread_info -> ptr -> WithPrePost@{X Z Y} Σ)
-  : function_spec Σ :=
+  Definition SDestructor@{X Z Y} (class : globname)
+             (PQ : ptr -> WithPrePost@{X Z Y} mpredI)
+  : function_spec :=
     let map_pre this '(args, P) := (Vptr this :: args, P) in
-    let map_post this '({| we_ex := pwiths ; we_post := Q|}) :=
+    let map_post this '{| we_ex := pwiths ; we_post := Q|} :=
         {| we_ex := pwiths
          ; we_post := tele_map (fun '(result, Q) =>
                                   (result, _at (_eq this) (anyR (Tnamed class) 1) ** Q)) Q |}
     in
     let this_type := Qmut (Tnamed class) in
-    TSFunction@{X Z Y} (Qmut Tvoid) (Qconst (Tpointer this_type) :: nil)
-               (fun ti =>
-                 {| wpp_with := TeleS (fun this : ptr => (PQ ti this).(wpp_with))
-                  ; wpp_pre this :=
-                       tele_map (map_pre this) (PQ ti this).(wpp_pre)
-                  ; wpp_post this :=
-                       tele_map (map_post this) (PQ ti this).(wpp_post)
-                  |}).
-
-  Definition SDestructor@{X Z Y} (class : globname) (PQ : ptr -> WithPrePost@{X Z Y} Σ)
-  : function_spec Σ := TSDestructor class (fun _ => PQ).
+    SFunction@{X Z Y} (Qmut Tvoid) (Qconst (Tpointer this_type) :: nil)
+              {| wpp_with := TeleS (fun this : ptr => (PQ this).(wpp_with))
+               ; wpp_pre this :=
+                   tele_map (map_pre this) (PQ this).(wpp_pre)
+               ; wpp_post this :=
+                   tele_map (map_post this) (PQ this).(wpp_post)
+              |}.
 
   (* Hoare triple for a method.
    *)
-  Definition TSMethod@{X Z Y} (class : globname) (qual : type_qualifiers)
+  Definition SMethod@{X Z Y} (class : globname) (qual : type_qualifiers)
              (ret : type) (targs : list type)
-             (PQ : thread_info -> ptr -> WithPrePost@{X Z Y} Σ)
-  : function_spec Σ :=
+             (PQ : ptr -> WithPrePost@{X Z Y} mpredI)
+  : function_spec :=
     let map_pre this '(args, P) := (this :: args, P) in
     let class_type := Tnamed class in
     let this_type := Tqualified qual class_type in
-    TSFunction ret (Qconst (Tpointer this_type) :: targs)
-               (fun ti =>
-                  {| wpp_with := TeleS (fun this : ptr => (PQ ti this).(wpp_with))
-                   ; wpp_pre this :=
-                       tele_map (map_pre (Vptr this)) (PQ ti this).(wpp_pre)
-                   ; wpp_post this := (PQ ti this).(wpp_post)
-                   |}).
+    SFunction ret (Qconst (Tpointer this_type) :: targs)
+              {| wpp_with := TeleS (fun this : ptr => (PQ this).(wpp_with))
+               ; wpp_pre this :=
+                   tele_map (map_pre (Vptr this)) (PQ this).(wpp_pre)
+               ; wpp_post this := (PQ this).(wpp_post)
+               |}.
       (* ^ todo(gmm): this looks wrong. something isn't going
        * to fit together with respect to calling conventions and
        * specifications.
        *)
 
-  Definition SMethod@{X Z Y} (class : globname) (qual : type_qualifiers)
-             (ret : type) (targs : list type)
-             (PQ : ptr -> WithPrePost@{X Z Y} Σ)
-  : function_spec Σ := TSMethod class qual ret targs (fun _ => PQ).
-
-  Local Definition local_addr_v (r : region) (x : ident) (v : val) : mpred Σ :=
+  Local Definition local_addr_v (r : region) (x : ident) (v : val) : mpred :=
     Exists p, [| v = Vptr p |] ** local_addr r x p.
 
-  Fixpoint bind_type ρ (t : type) (x : ident) (v : val) : mpred Σ :=
+  Fixpoint bind_type ρ (t : type) (x : ident) (v : val) : mpred :=
     match t with
     | Tqualified _ t => bind_type ρ t x v
     | Treference ref => local_addr_v ρ x v
     | Trv_reference ref => local_addr_v ρ x v
-    | Tnamed _         => local_addr_v ρ x v
-    | _              => tlocal ρ x (primR (erase_qualifiers t) 1 v)
+    | Tnamed _       => local_addr_v ρ x v
+    | _              => Exists a, tlocal_at ρ x a (primR (erase_qualifiers t) 1 v)
     end.
 
-  Fixpoint free_type ρ (t : type) (x : ident) (v : val) : mpred Σ :=
+  Fixpoint free_type ρ (t : type) (x : ident) (v : val) : mpred :=
     match t with
     | Tqualified _ t => free_type ρ t x v
     | Treference ref => local_addr_v ρ x v
     | Trv_reference ref => local_addr_v ρ x v
-    | Tnamed cls       => local_addr_v ρ x v
-    | _              => tlocal ρ x (anyR (erase_qualifiers t) 1)
+    | Tnamed cls     => local_addr_v ρ x v
+    | _              => Exists a, tlocal_at ρ x a (anyR (erase_qualifiers t) 1)
     end.
 
-  Fixpoint ForallEaches (ts : list type) : (list (type * val) -> mpred Σ) -> mpred Σ :=
+  Fixpoint ForallEaches (ts : list type) : (list (type * val) -> mpred) -> mpred :=
     match ts with
     | nil => fun k => k nil
     | t :: ts => fun k => Forall v : val, ForallEaches ts (fun args => k ((t,v) :: args))
@@ -220,9 +214,8 @@ Module Type Func.
     (* the proof obligation for a function
      *)
 
-  Definition wp_func (f : Func) (ti : thread_info) (args : list val) (Q : val -> epred Σ) : mpred Σ.
-  refine (
-      match f.(f_body) with
+  Definition wp_func (f : Func) (ti : thread_info) (args : list val) (Q : val -> epred) : mpred :=
+    match f.(f_body) with
       | None => lfalse
       | Some body =>
         let ret := f.(f_return) in
@@ -245,11 +238,9 @@ Module Type Func.
         else
           binds -*
           wp (resolve:=resolve) ti ρ body (Kfree frees (val_return (fun x => |> Q x)))
-      end).
-  Defined.
+      end.
 
-    Definition wp_method (meth : Method) (ti : thread_info) (args : list val) (Q : val -> epred Σ) : mpred Σ.
-    refine
+  Definition wp_method (meth : Method) ti (args : list val) (Q : val -> epred) : mpred :=
       match meth.(m_body) with
       | None => lfalse
       | Some body =>
@@ -281,16 +272,19 @@ Module Type Func.
           | _ => lfalse
           end
       end.
-    Defined.
     (* ^ todo(gmm): move the [frees] to the left hand side of the [-*], this
      * will make the right-hand-side more canonical
      *)
 
     (* todo(gmm): i should be able to define this using [wp_func] *)
-    Definition func_ok (ret : type) (params : list (ident * type))
-               (body : Stmt)
-               (ti : thread_info) (spec : function_spec Σ)
-    : mpred Σ :=
+    Definition func_ok (f : Func)
+               (ti : thread_info) (spec : function_spec)
+    : mpred :=
+      match f.(f_body) with
+      | None => lfalse
+      | Some body =>
+        let params := f.(f_params) in
+        let ret := f.(f_return) in
       [| type_of_spec spec = normalize_type (Tfunction ret (List.map snd params)) |] **
       (* forall each argument, apply to [fs_spec ti] *)
       ForallEaches (spec.(fs_arguments)) (fun args =>
@@ -307,25 +301,26 @@ Module Type Func.
                    (rev params) (rev vals)) in
         if is_void ret
         then
-          Forall Q : mpred Σ,
+          Forall Q : mpred,
           (binds ** PQ (fun x => Q)) -*
           wp (resolve:=resolve) ti ρ body (Kfree frees (void_return (|>Q)))
         else if is_aggregate ret then
-          Forall Q : val -> mpred Σ,
+          Forall Q : val -> mpred,
           Forall ra,
           (binds ** result_addr ρ ra ** _at (_eq ra) (uninitR (erase_qualifiers ret) 1) ** PQ Q) -*
           wp (resolve:=resolve) ti ρ body (Kfree (frees ** result_addr ρ ra) (val_return (fun x => |> Q x)))
         else
-          Forall Q : val -> mpred Σ,
+          Forall Q : val -> mpred,
           (binds ** PQ Q) -*
-          wp (resolve:=resolve) ti ρ body (Kfree frees (val_return (fun x => |> Q x)))).
+          wp (resolve:=resolve) ti ρ body (Kfree frees (val_return (fun x => |> Q x))))
+      end.
     (* ^ todo(gmm): the new semantics of function gets an address for a return value
      * so the semantics for `return` should be that *)
 
 
 
-    Definition method_ok (meth : Method) (ti : thread_info) (spec : function_spec Σ)
-      : mpred Σ :=
+    Definition method_ok (meth : Method) (ti : thread_info) (spec : function_spec)
+      : mpred :=
       match meth.(m_body) with
       | None => lfalse
       | Some body =>
@@ -355,14 +350,14 @@ Module Type Func.
             let ret_ty := meth.(m_return) in
             if is_void ret_ty
             then
-              Forall Q : mpred Σ,
+              Forall Q : mpred,
               (binds ** PQ (fun x => Q)) -* (wp (resolve:=resolve) ti ρ body (Kfree frees (void_return (|>Q))))
             else if is_aggregate ret_ty then
-              Forall Q : val -> mpred Σ,
+              Forall Q : val -> mpred,
               Forall ra,
               (binds ** result_addr ρ ra ** _at (_eq ra) (uninitR (erase_qualifiers ret_ty) 1) ** PQ Q) -* (wp (resolve:=resolve) ti ρ body (Kfree (frees ** result_addr ρ ra) (val_return (fun x => |>Q x))))
             else
-              Forall Q : val -> mpred Σ,
+              Forall Q : val -> mpred,
               (binds ** PQ Q) -* (wp (resolve:=resolve) ti ρ body (Kfree frees (val_return (fun x => |>Q x))))
           | _ => lfalse
           end)
@@ -371,9 +366,9 @@ Module Type Func.
      * will make the right-hand-side more canonical
      *)
 
-    Fixpoint wpis (ti : thread_info) (ρ : region)  (cls : globname) (this : val)
+    Fixpoint wpis (ti : thread_info) (ρ : region) (cls : globname) (this : val)
              (inits : list Initializer)
-             (Q : mpred Σ -> mpred Σ) : mpred Σ :=
+             (Q : mpred -> mpred) : mpred :=
       match inits with
       | nil => Q empSP
       | i :: is' => wpi (resolve:=resolve) ti ρ cls this i (fun f => f ** wpis ti ρ cls this is' Q)
@@ -383,14 +378,14 @@ Module Type Func.
     Definition wp_ctor (cls : globname) (ti : thread_info) (ρ : region)
                (this_val : val)
                (inits : list Initializer) (body : Stmt)
-               (Q : Kpreds Σ)
-    : mpred Σ :=
+               (Q : Kpreds)
+    : mpred :=
       wpis ti ρ cls this_val inits
            (fun free => free ** wp (resolve:=resolve) ti ρ body Q).
 
 
-    Definition ctor_ok (ctor : Ctor) ti (spec : function_spec Σ)
-    : mpred Σ :=
+    Definition ctor_ok (ctor : Ctor) (ti : thread_info) (spec : function_spec)
+    : mpred :=
       match ctor.(c_body) with
       | None => lfalse
       | Some Defaulted => lfalse
@@ -418,7 +413,7 @@ Module Type Func.
                 this_addr ρ thisp **
                 sepSPs (zip_with (fun '(x, t) 'v => free_type ρ t x v) (rev ctor.(c_params)) (rev rest_vals))
             in
-            Forall Q : mpred Σ,
+            Forall Q : mpred,
             (binds ** PQ (fun x => Q)) -*
             (wp_ctor ctor.(c_class) ti ρ (Vptr thisp) init body
                      (Kfree frees (void_return (|>Q))))
@@ -426,26 +421,26 @@ Module Type Func.
           end)
       end.
 
-    Fixpoint wpds ti ρ
+    Fixpoint wpds (ti : thread_info) (ρ : region)
              (cls : globname) (this : val)
              (dests : list (FieldOrBase * globname))
-             (Q : mpred Σ) : mpred Σ :=
+             (Q : mpred) : mpred :=
       match dests with
       | nil => Q
-      | d :: ds => @wpd Σ resolve ti ρ cls this d (wpds ti ρ cls this ds Q)
+      | d :: ds => @wpd _ Σ resolve ti ρ cls this d (wpds ti ρ cls this ds Q)
       end.
 
 
-    Definition wp_dtor (cls : globname) (ti : thread_info) (ρ : region)
+    Definition wp_dtor (ti : thread_info) (ρ : region) (cls : globname)
                (this_val : val)
                (body : Stmt) (dtors : list (FieldOrBase * globname))
-               (frees : mpred Σ) (Q : mpred Σ)
-    : mpred Σ :=
-      @wp Σ resolve ti ρ body
+               (frees : mpred) (Q : mpred)
+    : mpred :=
+      @wp _ Σ resolve ti ρ body
          (Kfree frees (void_return (wpds ti ρ cls this_val dtors Q))).
 
-    Definition dtor_ok (dtor : Dtor) ti (spec : function_spec Σ)
-    : mpred Σ :=
+    Definition dtor_ok (dtor : Dtor) (ti : thread_info) (spec : function_spec)
+    : mpred :=
       match dtor.(d_body) with
       | None => lfalse
       | Some Defaulted => lfalse
@@ -466,13 +461,13 @@ Module Type Func.
             let binds := this_addr ρ thisp in
             (* this is what is freed on return *)
             let frees := this_addr ρ thisp in
-            Forall Q : mpred Σ,
+            Forall Q : mpred,
               (binds ** PQ (fun x => Q)) -*
-              (wp_dtor dtor.(d_class) ti ρ (Vptr thisp) body deinit frees (|>Q))
+              (wp_dtor ti ρ dtor.(d_class) (Vptr thisp) body deinit frees (|>Q))
           | _ => lfalse
           end)
       end.
-  End with_Σ.
+  End with_cpp.
 
 End Func.
 
