theories/lang/cpp/logic/initializers.v
@@ -11,37 +11,33 @@ Local Open Scope Z_scope.
 Require Import bedrock.lang.cpp.ast.
 Require Import bedrock.lang.cpp.semantics.
 From bedrock.lang.cpp.logic Require Import
-     pred heap_pred call wp intensional.
+     pred path_pred heap_pred call wp intensional.
 
 Module Type Init.
 
   Section with_resolve.
-    Context {Σ:gFunctors} {resolve:genv}.
-    Variable ti : thread_info.
-    Variable ρ : region.
+    Context `{Σ : cpp_logic thread_info} {σ:genv}.
+    Variables (ti : thread_info) (ρ : region).
 
-    Local Notation wp := (wp (Σ :=Σ) (resolve:=resolve) ti ρ).
-    Local Notation wpi := (wpi (Σ :=Σ) (resolve:=resolve) ti ρ).
-    Local Notation wpe := (wpe (Σ :=Σ) (resolve:=resolve) ti ρ).
-    Local Notation wp_lval := (wp_lval (Σ :=Σ) (resolve:=resolve) ti ρ).
-    Local Notation wp_rval := (wp_rval (Σ :=Σ) (resolve:=resolve) ti ρ).
-    Local Notation wp_prval := (wp_prval (Σ :=Σ) (resolve:=resolve) ti ρ).
-    Local Notation wp_xval := (wp_xval (Σ :=Σ) (resolve:=resolve) ti ρ).
-    Local Notation wp_init := (wp_init (Σ :=Σ) (resolve:=resolve) ti ρ).
-    Local Notation wp_args := (wp_args (Σ :=Σ) (resolve:=resolve) ti ρ).
-    Local Notation fspec := (fspec (Σ :=Σ)).
+    Local Notation wp := (wp (resolve:=σ) ti ρ).
+    Local Notation wpi := (wpi (resolve:=σ) ti ρ).
+    Local Notation wpe := (wpe (resolve:=σ) ti ρ).
+    Local Notation wp_lval := (wp_lval (resolve:=σ) ti ρ).
+    Local Notation wp_rval := (wp_rval (resolve:=σ) ti ρ).
+    Local Notation wp_prval := (wp_prval (resolve:=σ) ti ρ).
+    Local Notation wp_xval := (wp_xval (resolve:=σ) ti ρ).
+    Local Notation wp_init := (wp_init (resolve:=σ) ti ρ).
+    Local Notation wp_args := (wp_args (σ:=σ) ti ρ).
+    Local Notation fspec := (fspec ti).
 
-    Local Notation _global := (@_global resolve) (only parsing).
-    Local Notation _field := (@_field resolve) (only parsing).
-    Local Notation _sub := (@_sub resolve) (only parsing).
-    Local Notation _super := (@_super resolve) (only parsing).
-    Local Notation primR := (@primR Σ resolve) (only parsing).
-    Local Notation offset_for := (@offset_for resolve) (only parsing).
-    Local Notation uninitR := (@uninitR Σ resolve) (only parsing).
+    Local Notation _global := (_global (resolve:=σ)) (only parsing).
+    Local Notation _field := (_field (resolve:=σ)) (only parsing).
+    Local Notation _sub := (_sub (resolve:=σ)) (only parsing).
+    Local Notation _super := (_super (resolve:=σ)) (only parsing).
+    Local Notation primR := (primR (resolve:=σ)) (only parsing).
+    Local Notation offset_for := (offset_for σ) (only parsing).
+    Local Notation uninitR := (uninitR (resolve:=σ)) (only parsing).
 
-
-    Local Notation mpred := (mpred Σ) (only parsing).
-    Local Notation FreeTemps := (FreeTemps Σ) (only parsing).
 
     (* this is really about expression evaluation, so it doesn't make sense for
      * it to be recursive on a type.
@@ -91,7 +87,7 @@ Module Type Init.
     Axiom wp_init_constructor : forall cls addr cnd es Q ty,
       wp_args es (fun ls free =>
          Exists ctor, _global cnd &~ ctor **
-         |> fspec (Vptr ctor) ti (addr :: ls) (fun _ => Q free))
+         |> fspec (Vptr ctor) (addr :: ls) (fun _ => Q free))
       |-- wp_init (Tnamed cls) addr (Econstructor cnd es ty) Q.
 
     Definition build_array (es : list Expr) (fill : option Expr) (sz : nat)
