theories/lang/cpp/logic/layout.v
@@ -8,20 +8,19 @@ Require Import Coq.ZArith.BinInt.
 
 Require Import bedrock.lang.cpp.ast.
 From bedrock.lang.cpp.logic Require Import
-     pred heap_pred compilation_unit.
+     pred path_pred heap_pred compilation_unit.
 Require Import bedrock.lang.cpp.semantics.
 
 Section with_Σ.
-  Context {Σ : gFunctors} {resolve:genv}.
+  Context `{Σ : cpp_logic ti} {resolve:genv}.
 
-  Local Notation mpred := (mpred Σ) (only parsing).
   Local Notation _super := (_super (resolve:=resolve)) (only parsing).
   Local Notation _field := (_field (resolve:=resolve)) (only parsing).
   Local Notation _sub := (_sub (resolve:=resolve)) (only parsing).
-  Local Notation uninitR := (uninitR (Σ:=Σ) (resolve:=resolve)) (only parsing).
-  Local Notation anyR := (anyR (Σ:=Σ) (resolve:=resolve)) (only parsing).
+  Local Notation uninitR := (uninitR (resolve:=resolve)) (only parsing).
+  Local Notation anyR := (anyR (resolve:=resolve)) (only parsing).
 
-Axiom uninit_class_fwd
+  Axiom uninit_class_fwd
   : forall cls base st q,
     glob_def resolve cls = Some (Gstruct st) ->
     _at (Σ:=Σ) (_eqv base) (uninitR (Tnamed cls) q)
@@ -36,8 +35,8 @@ Axiom uninit_class_fwd
                                    (_field {| f_name := n ; f_type := cls |})
                                    (uninitR (erase_qualifiers t) q)) st.(s_fields))).
 
-Axiom anyR_class_bwd
-: forall cls base st q,
+  Axiom anyR_class_bwd
+  : forall cls base st q,
     glob_def resolve cls = Some (Gstruct st) ->
     _at (_eqv base)
         (sepSPs (List.map (fun '(gn,_) =>
@@ -47,11 +46,11 @@ Axiom anyR_class_bwd
                                       (anyR (erase_qualifiers t) q)) st.(s_fields)))
     |-- _at (Σ:=Σ) (_eqv base) (anyR (Tnamed cls) q).
 
-Axiom uninit_array : forall t n q,
+  Axiom uninit_array : forall t n q,
     uninitR (Tarray t n) q
     -|- sepSPs (map (fun i => _offsetR (_sub t (Z.of_nat i)) (uninitR t q)) (seq 0 (BinNatDef.N.to_nat n))).
 
-Axiom anyR_array : forall t n q,
+  Axiom anyR_array : forall t n q,
     anyR (Tarray t n) q
     -|- sepSPs (map (fun i => _offsetR (_sub t (Z.of_nat i)) (anyR t q)) (seq 0 (BinNatDef.N.to_nat n))).
 End with_Σ.
