theories/lang/cpp/logic/path_pred.v
@@ -1,0 +1,207 @@
+(*
+ * Copyright (C) BedRock Systems Inc. 2019 Gregory Malecha
+ *
+ * SPDX-License-Identifier:AGPL-3.0-or-later
+ *)
+Require Import Coq.Classes.Morphisms.
+Require Import Coq.NArith.BinNat.
+Require Import Coq.ZArith.BinInt.
+Require Import Coq.Strings.String.
+
+From iris.bi Require Export monpred.
+
+From bedrock.lang.cpp Require Import semantics logic.pred ast.
+
+Local Open Scope string_scope.
+
+Lemma monPred_at_persistent_inv {V bi} (P : monPred V bi) :
+  (∀ i, Persistent (P i)) → Persistent P.
+Proof. intros HP. constructor=> i. MonPred.unseal. apply HP. Qed.
+
+Lemma monPred_at_timeless_inv {V sbi} (P : monPredSI V sbi) :
+  (∀ i, Timeless (P i)) → Timeless P.
+Proof. intros HP. constructor=> i. MonPred.unseal. apply HP. Qed.
+
+Section with_Σ.
+  Context `{has_cpp : cpp_logic ti}.
+
+  (* locations are computations that produce an address.
+   * - note(gmm): they are always computable from the program except.
+   *)
+  Definition Loc : Type := option ptr.
+
+  Definition Offset : Type := option (ptr -> option ptr).
+
+  Local Ltac solve_Loc_persistent X :=
+    intros;
+    rewrite X;
+    constructor; apply monPred_at_persistent_inv;
+    apply _.
+  Local Ltac solve_Offset_persistent X :=
+    intros;
+    rewrite X;
+    constructor; apply monPred_at_persistent_inv;
+    constructor; apply monPred_at_persistent_inv;
+    apply _.
+
+  Local Ltac solve_Loc_timeless X :=
+    intros;
+    rewrite X;
+    constructor; apply monPred_at_timeless_inv;
+    apply _.
+  Local Ltac solve_Offset_timeless X :=
+    intros;
+    rewrite X;
+    constructor; apply monPred_at_timeless_inv;
+    constructor; apply monPred_at_timeless_inv;
+    apply _.
+
+  Definition LocEq (l1 l2 : Loc) : Prop :=
+    l1 = l2.
+
+  Definition this_addr (r : region) (p : ptr) : mpred :=
+    local_addr r "#this" p.
+
+  Definition result_addr (r : region) (p : ptr) : mpred :=
+    local_addr r "#result" p.
+
+  (* absolute locations *)
+  Definition _eq_def (p : ptr) : Loc :=
+    Some p.
+  Definition _eq_aux : seal (@_eq_def). by eexists. Qed.
+  Definition _eq := _eq_aux.(unseal).
+  Definition _eq_eq : @_eq = _ := _eq_aux.(seal_eq).
+
+
+  Definition _eqv (a : val) : Loc :=
+    match a with
+    | Vptr p => _eq p
+    | _ => None
+    end.
+
+  Lemma _eqv_eq : forall p, _eqv (Vptr p) = _eq p.
+  Proof. reflexivity. Qed.
+
+  (* ^ these two could be duplicable because regions don't need to be
+   * reused. the reason that local variables need to be tracked is that
+   * they could go out of scope.
+   * - an alternative, and (sound) solution is to generate a fresh region
+   *   each time that we create a new scope. To do this, we need to track in
+   *   the AST the debruijn index of the binder.
+   * - yet another alternative is to inline regions explicitly into the WP.
+   *   essentially region := list (list (string * ptr)). this essentially makes
+   *   _local persistent.
+   *)
+
+  Definition _global_def (resolve : genv) (x : obj_name) : Loc :=
+    match glob_addr resolve x with
+    | None => None
+    | Some p => Some p
+    end.
+  Definition _global_aux : seal (@_global_def). by eexists. Qed.
+  Definition _global := _global_aux.(unseal).
+  Definition _global_eq : @_global = _ := _global_aux.(seal_eq).
+
+  (* offsets *)
+  Definition _field_def (resolve: genv) (f : field) : Offset :=
+    match offset_of resolve f.(f_type) f.(f_name) with
+    | Some o => Some (fun p => Some (offset_ptr_ o p))
+    | _ => None
+    end.
+  Definition _field_aux : seal (@_field_def). Proof using. by eexists. Qed.
+  Definition _field := _field_aux.(unseal).
+  Definition _field_eq : @_field = _ := _field_aux.(seal_eq).
+
+  Definition _sub_def (resolve:genv) (t : type) (i : Z) : Offset :=
+    match size_of resolve t with
+    | Some n => Some (fun p => Some (offset_ptr_ (i * Z.of_N n) p))
+    | _ => None
+    end.
+  Definition _sub_aux : seal (@_sub_def). by eexists. Qed.
+  Definition _sub := _sub_aux.(unseal).
+  Definition _sub_eq : @_sub = _ := _sub_aux.(seal_eq).
+
+
+  (* this represents static_cast *)
+  Definition _super_def (resolve:genv) (sub super : globname) : Offset :=
+    match parent_offset resolve sub super with
+    | Some o => Some (fun p => Some (offset_ptr_ o p))
+    | _ => None
+    end.
+  Definition _super_aux : seal (@_super_def). by eexists. Qed.
+  Definition _super := _super_aux.(unseal).
+  Definition _super_eq : @_super = _ := _super_aux.(seal_eq).
+
+  Definition _id_def : Offset := Some (fun x => Some x).
+  Definition _id_aux : seal (@_id_def). by eexists. Qed.
+  Definition _id := _id_aux.(unseal).
+  Definition _id_eq : @_id = _ := _id_aux.(seal_eq).
+
+  Definition _dot_def (o1 o2 : Offset) : Offset :=
+    match o1 , o2 with
+    | Some o1 , Some o2 => Some (fun x => match o1 x with
+                                      | None => None
+                                      | Some p => o2 p
+                                      end)
+    | _ , _ => None
+    end.
+  Definition _dot_aux : seal (@_dot_def). by eexists. Qed.
+  Definition _dot := _dot_aux.(unseal).
+  Definition _dot_eq : @_dot = _ := _dot_aux.(seal_eq).
+
+  Definition _offsetL_def (o : Offset) (l : Loc) : Loc :=
+    match o , l with
+    | Some o , Some l => match o l with
+                        | None => None
+                        | Some p => Some p
+                        end
+    | _ , _ => None
+    end.
+  Definition _offsetL_aux : seal (@_offsetL_def). by eexists. Qed.
+  Definition _offsetL := _offsetL_aux.(unseal).
+  Definition _offsetL_eq : @_offsetL = _ := _offsetL_aux.(seal_eq).
+
+
+  Definition addr_of_def (a : Loc) (b : ptr) : mpred :=
+    [| a = Some b |].
+  Definition addr_of_aux : seal (@addr_of_def). by eexists. Qed.
+  Definition addr_of := addr_of_aux.(unseal).
+  Definition addr_of_eq : @addr_of = _ := addr_of_aux.(seal_eq).
+  Arguments addr_of : simpl never.
+  Notation "a &~ b" := (addr_of a b) (at level 30, no associativity).
+
+  Global Instance addr_of_persistent : Persistent (addr_of o l).
+  Proof. rewrite addr_of_eq. apply _. Qed.
+
+
+  (* this is for `Indirect` field references *)
+  Fixpoint path_to_Offset (resolve:genv) (from : globname) (final : ident)
+           (ls : list (ident * globname))
+    : Offset :=
+    match ls with
+    | nil => @_field resolve {| f_type := from ; f_name := final |}
+    | cons (i,c) ls =>
+      _dot (@_field resolve {| f_type := from ; f_name := i |}) (path_to_Offset resolve c final ls)
+    end.
+
+  Definition offset_for (resolve:genv) (cls : globname) (f : FieldOrBase) : Offset :=
+    match f with
+    | Base parent => _super resolve cls parent
+    | Field i => _field resolve {| f_type := cls ; f_name := i |}
+    | Indirect ls final =>
+      path_to_Offset resolve cls final ls
+    | This => _id
+    end.
+
+End with_Σ.
+
+Arguments addr_of : simpl never.
+Notation "a &~ b" := (addr_of a b) (at level 30, no associativity).
+
+Global Opaque _sub _field _offsetL _dot addr_of.
+Global Opaque this_addr result_addr.
+
+Arguments _super {resolve} _ _ : rename.
+Arguments _field {resolve} _ : rename.
+Arguments _sub {resolve} _ : rename.
+Arguments _global {resolve} _ : rename.
